TestVectorsAwsCryptographicMaterialProviders/runtimes/net/Generated/KeyVectors/CachingCMM.cs
@@ -1,0 +1,77 @@
+// Copyright Amazon.com Inc. or its affiliates. All Rights Reserved.
+// SPDX-License-Identifier: Apache-2.0
+// Do not modify this file. This file is machine generated, and any changes to it will be overwritten.
+using System;
+using AWS.Cryptography.MaterialProvidersTestVectorKeys;
+namespace AWS.Cryptography.MaterialProvidersTestVectorKeys
+{
+  public class CachingCMM
+  {
+    private AWS.Cryptography.MaterialProvidersTestVectorKeys.KeyDescription _underlying;
+    private int? _cacheLimitTtlSeconds;
+    private long? _limitBytes;
+    private int? _limitMessages;
+    private System.IO.MemoryStream _getEntryIdentifier;
+    private System.IO.MemoryStream _putEntryIdentifier;
+    public AWS.Cryptography.MaterialProvidersTestVectorKeys.KeyDescription Underlying
+    {
+      get { return this._underlying; }
+      set { this._underlying = value; }
+    }
+    public bool IsSetUnderlying()
+    {
+      return this._underlying != null;
+    }
+    public int CacheLimitTtlSeconds
+    {
+      get { return this._cacheLimitTtlSeconds.GetValueOrDefault(); }
+      set { this._cacheLimitTtlSeconds = value; }
+    }
+    public bool IsSetCacheLimitTtlSeconds()
+    {
+      return this._cacheLimitTtlSeconds.HasValue;
+    }
+    public long LimitBytes
+    {
+      get { return this._limitBytes.GetValueOrDefault(); }
+      set { this._limitBytes = value; }
+    }
+    public bool IsSetLimitBytes()
+    {
+      return this._limitBytes.HasValue;
+    }
+    public int LimitMessages
+    {
+      get { return this._limitMessages.GetValueOrDefault(); }
+      set { this._limitMessages = value; }
+    }
+    public bool IsSetLimitMessages()
+    {
+      return this._limitMessages.HasValue;
+    }
+    public System.IO.MemoryStream GetEntryIdentifier
+    {
+      get { return this._getEntryIdentifier; }
+      set { this._getEntryIdentifier = value; }
+    }
+    public bool IsSetGetEntryIdentifier()
+    {
+      return this._getEntryIdentifier != null;
+    }
+    public System.IO.MemoryStream PutEntryIdentifier
+    {
+      get { return this._putEntryIdentifier; }
+      set { this._putEntryIdentifier = value; }
+    }
+    public bool IsSetPutEntryIdentifier()
+    {
+      return this._putEntryIdentifier != null;
+    }
+    public void Validate()
+    {
+      if (!IsSetUnderlying()) throw new System.ArgumentException("Missing value for required property 'Underlying'");
+      if (!IsSetCacheLimitTtlSeconds()) throw new System.ArgumentException("Missing value for required property 'CacheLimitTtlSeconds'");
+
+    }
+  }
+}
