TestVectorsAwsCryptographicMaterialProviders/dafny/KeyVectors/src/CmmFromKeyDescription.dfy
@@ -1,0 +1,133 @@
+// Copyright Amazon.com Inc. or its affiliates. All Rights Reserved.
+// SPDX-License-Identifier: Apache-2.0
+
+include "../Model/AwsCryptographyMaterialProvidersTestVectorKeysTypes.dfy"
+  // Yes this is including from somewhere else.
+include "../../TestVectorsAwsCryptographicMaterialProviders/src/LibraryIndex.dfy"
+include "KeyringFromKeyDescription.dfy"
+include "CreateStaticCMCs.dfy"
+
+module {:options "-functionSyntax:4"} CmmFromKeyDescription {
+  import opened Types = AwsCryptographyMaterialProvidersTestVectorKeysTypes
+  import MPL = AwsCryptographyMaterialProvidersTypes
+  import opened Wrappers
+  import KeyringFromKeyDescription
+  import CreateStaticCMCs
+  import UTF8
+
+  method ToCmm(
+    mpl: MPL.IAwsCryptographicMaterialProvidersClient,
+    info: KeyringFromKeyDescription.KeyringInfo,
+    forOperation: CmmOperation
+  )
+    returns (output: Result<MPL.ICryptographicMaterialsManager, Error>)
+    requires mpl.ValidState()
+    modifies mpl.Modifies
+    decreases info.description
+    ensures mpl.ValidState()
+    ensures output.Success? ==>
+              && output.value.ValidState()
+              && fresh(output.value.Modifies - mpl.Modifies)
+              && output.value.Modifies !! {mpl.History}
+  {
+    var KeyringInfo(description, material) := info;
+
+    match description
+    case RequiredEncryptionContext(cmm) => {
+      var underlying :- ToCmm(mpl, info.( description := cmm.underlying ), forOperation);
+      var output' := mpl
+      .CreateRequiredEncryptionContextCMM(
+        MPL.CreateRequiredEncryptionContextCMMInput(
+          underlyingCMM := Some(underlying),
+          keyring := None,
+          requiredEncryptionContextKeys := cmm.requiredEncryptionContextKeys
+        )
+      );
+      output := output'.MapFailure(e => Types.AwsCryptographyMaterialProviders(e));
+    }
+    case Caching(cmm) => {
+
+      var identifier := if cmm.getEntryIdentifier.Some? && cmm.putEntryIdentifier.Some? then
+        Some(CreateStaticCMCs.Identifiers(
+               getIdentifier := cmm.getEntryIdentifier.value,
+               putIdentifier := cmm.putEntryIdentifier.value
+             ))
+      else if cmm.getEntryIdentifier.Some? then
+        Some(CreateStaticCMCs.Identifier.GetIdentifier(
+               identifier := cmm.getEntryIdentifier.value
+             ))
+      else if cmm.getEntryIdentifier.Some? then
+        Some(CreateStaticCMCs.PutIdentifier(
+               identifier := cmm.putEntryIdentifier.value
+             ))
+      else
+        None;
+
+      :- Need(identifier.Some? ==> material.Some? && material.value.StaticMaterial?,
+              KeyVectorException( message := "CachingCMM only supports StaticMaterial."));
+      var underlying :- ToCmm(mpl, info.( description := cmm.underlying ), forOperation);
+
+
+
+      var entry := if identifier.Some? then
+        match forOperation
+        case ENCRYPT() =>
+          Some(CreateStaticCMCs.StaticCMCEntry(
+                 materials := MPL.Materials.Encryption(
+                   MPL.EncryptionMaterials(
+                     algorithmSuite := material.value.algorithmSuite,
+                     encryptedDataKeys := material.value.encryptedDataKeys,
+                     encryptionContext := material.value.encryptionContext,
+                     requiredEncryptionContextKeys := material.value.requiredEncryptionContextKeys,
+                     plaintextDataKey := material.value.plaintextDataKey,
+                     signingKey := material.value.signingKey,
+                     symmetricSigningKeys := material.value.symmetricSigningKeys
+                   )),
+                 identifier := identifier.value
+               ))
+        case DECRYPT() =>
+          Some(CreateStaticCMCs.StaticCMCEntry(
+                 materials := MPL.Materials.Decryption(
+                   MPL.DecryptionMaterials(
+                     algorithmSuite := material.value.algorithmSuite,
+                     encryptionContext := material.value.encryptionContext,
+                     requiredEncryptionContextKeys := material.value.requiredEncryptionContextKeys,
+                     plaintextDataKey := material.value.plaintextDataKey,
+                     verificationKey := material.value.verificationKey,
+                     symmetricSigningKey := None // need to pass one vs many :(
+                   )),
+                 identifier := identifier.value
+               ))
+      else
+        None;
+
+      var underlyingCMC := CreateStaticCMCs.CreateStaticCMC(entry);
+      var partitionKey :- expect UTF8.Encode("asdf");
+
+      var createCachingCMMInput
+        := MPL.CreateCachingCMMInput(
+        underlyingCMM := Some(underlying),
+        keyring := None,
+        underlyingCMC := underlyingCMC,
+        cacheLimitTtlSeconds := cmm.cacheLimitTtlSeconds,
+        partitionKey := Some(partitionKey), // String "asdf" in UTF8 bytes
+        limitBytes := cmm.limitBytes,
+        limitMessages := cmm.limitMessages
+      );
+
+      var output' := mpl.CreateCachingCMM(createCachingCMMInput);
+      output := output'.MapFailure(e => Types.AwsCryptographyMaterialProviders(e));
+
+      assert createCachingCMMInput.underlyingCMC is CreateStaticCMCs.StaticCMC;
+    }
+    case _ => {
+      var keyring :- KeyringFromKeyDescription.ToKeyring(mpl, info);
+      var output' := mpl
+      .CreateDefaultCryptographicMaterialsManager(
+        MPL.CreateDefaultCryptographicMaterialsManagerInput( keyring := keyring )
+      );
+      output := output'.MapFailure(e => Types.AwsCryptographyMaterialProviders(e));
+    }
+  }
+
+}
