TestVectorsAwsCryptographicMaterialProviders/dafny/KeyVectors/src/CreateStaticCMCs.dfy
@@ -1,0 +1,207 @@
+// Copyright Amazon.com Inc. or its affiliates. All Rights Reserved.
+// SPDX-License-Identifier: Apache-2.0
+
+include "../Model/AwsCryptographyMaterialProvidersTestVectorKeysTypes.dfy"
+include "KeyMaterial.dfy"
+
+module {:options "-functionSyntax:4"} CreateStaticCMCs {
+  import opened AwsCryptographyMaterialProvidersTypes
+  import opened Wrappers
+  import opened StandardLibrary.UInt
+  import KeyMaterial
+  import Time
+
+  datatype Identifier =
+    | GetIdentifier(
+        identifier: seq<uint8>
+      )
+    | PutIdentifier(
+        identifier: seq<uint8>
+      )
+    | Identifiers (
+        getIdentifier: seq<uint8>,
+        putIdentifier: seq<uint8>
+      )
+
+  datatype StaticCMCEntry = StaticCMCEntry (
+    materials: Materials,
+    identifier: Identifier
+  )
+
+  method CreateStaticCMC(
+    entry : Option<StaticCMCEntry>
+  )
+    returns (cmc: ICryptographicMaterialsCache)
+    // requires staticKeyMaterial.StaticMaterial?
+    ensures
+      && cmc.ValidState()
+      && fresh(cmc) && fresh(cmc.Modifies)
+      && cmc.Modifies == {cmc.History}
+      && cmc is StaticCMC
+  {
+    return new StaticCMC(entry);
+  }
+
+  class StaticCMC extends ICryptographicMaterialsCache
+    {
+    constructor( entry : Option<StaticCMCEntry>)
+      ensures
+        && ValidState()
+        && fresh(History)
+        && fresh(Modifies)
+    {
+
+      staticEntry := entry;
+      History := new ICryptographicMaterialsCacheCallHistory();
+      Modifies := {History};
+    }
+
+    const staticEntry: Option<StaticCMCEntry>
+
+    function GetIdentifier()
+      : Option<seq<uint8>>
+    {
+      if staticEntry.Some? then
+        match staticEntry.value.identifier
+        case GetIdentifier(g) => Some(g)
+        case Identifiers(g,_) => Some(g)
+        case PutIdentifier(_) => Wrappers.None
+      else
+        Wrappers.None
+    }
+
+    function PutIdentifier()
+      : Option<seq<uint8>>
+    {
+      if staticEntry.Some? then
+        match staticEntry.value.identifier
+        case GetIdentifier(_) => Wrappers.None
+        case Identifiers(_,p) => Some(p)
+        case PutIdentifier(p) => Some(p)
+      else
+        Wrappers.None
+    }
+
+
+    ghost predicate ValidState()
+      reads this`Modifies, Modifies - {History}
+      ensures ValidState() ==> History in Modifies
+    {
+      && Modifies == {History}
+    }
+
+    // These are the supported Static information
+
+    ghost predicate PutCacheEntryEnsuresPublicly(input: PutCacheEntryInput , output: Result<(), Error>)
+    {true}
+
+    method PutCacheEntry' ( input: PutCacheEntryInput )
+      returns (output: Result<(), Error>)
+      requires
+        && ValidState()
+      modifies Modifies - {History}
+      // Dafny will skip type parameters when generating a default decreases clause.
+      decreases Modifies - {History}
+      ensures
+        && ValidState()
+      ensures PutCacheEntryEnsuresPublicly(input, output)
+      ensures unchanged(History)
+    {
+      var identifier := PutIdentifier();
+      if identifier.Some? {
+        expect input.identifier == identifier.value;
+      }
+      output := Success(());
+    }
+
+    ghost predicate GetCacheEntryEnsuresPublicly(input: GetCacheEntryInput , output: Result<GetCacheEntryOutput, Error>)
+    {true}
+
+    method GetCacheEntry' ( input: GetCacheEntryInput )
+      returns (output: Result<GetCacheEntryOutput, Error>)
+      requires
+        && ValidState()
+      modifies Modifies - {History}
+      // Dafny will skip type parameters when generating a default decreases clause.
+      decreases Modifies - {History}
+      ensures
+        && ValidState()
+      ensures GetCacheEntryEnsuresPublicly(input, output)
+      ensures unchanged(History)
+    {
+
+      var identifier := GetIdentifier();
+      if identifier.Some? {
+        expect input.identifier == identifier.value;
+
+        var now := Time.GetCurrent();
+        var range: BoundedInts.int64 := 10;
+
+        expect 0 < now - range;
+        expect now < INT64_MAX_LIMIT as BoundedInts.int64  - range;
+
+        var creationTime := now - range; // always in the past;
+        var expiryTime := now + range; // alway in the future;
+
+        output := Success(
+          GetCacheEntryOutput(
+            materials := staticEntry.value.materials,
+            creationTime := creationTime,
+            expiryTime := expiryTime,
+            messagesUsed := range as BoundedInts.int32,
+            bytesUsed := range
+          )
+        );
+      } else {
+        output := Failure(EntryDoesNotExist(message := "Entry does not exist"));
+      }
+    }
+
+
+
+    // These are all not supported operations in a static context
+
+    ghost predicate UpdateUsageMetadataEnsuresPublicly(input: UpdateUsageMetadataInput , output: Result<(), Error>)
+    {true}
+
+    method UpdateUsageMetadata' ( input: UpdateUsageMetadataInput )
+      returns (output: Result<(), Error>)
+      requires
+        && ValidState()
+      modifies Modifies - {History}
+      // Dafny will skip type parameters when generating a default decreases clause.
+      decreases Modifies - {History}
+      ensures
+        && ValidState()
+      ensures UpdateUsageMetadataEnsuresPublicly(input, output)
+      ensures unchanged(History)
+    {
+      output := Failure(
+        AwsCryptographicMaterialProvidersException(
+          message := "UpdateUsageMetadata is not supported for StaticCMC"
+        ));
+    }
+
+    ghost predicate DeleteCacheEntryEnsuresPublicly(input: DeleteCacheEntryInput , output: Result<(), Error>)
+    {true}
+
+    method DeleteCacheEntry' ( input: DeleteCacheEntryInput )
+      returns (output: Result<(), Error>)
+      requires
+        && ValidState()
+      modifies Modifies - {History}
+      // Dafny will skip type parameters when generating a default decreases clause.
+      decreases Modifies - {History}
+      ensures
+        && ValidState()
+      ensures DeleteCacheEntryEnsuresPublicly(input, output)
+      ensures unchanged(History)
+    {
+      output := Failure(
+        AwsCryptographicMaterialProvidersException(
+          message := "DeleteCacheEntry is not supported for StaticCMC"
+        ));
+    }
+
+  }
+}
