TestVectorsAwsCryptographicMaterialProviders/dafny/TestVectorsAwsCryptographicMaterialProviders/src/VectorsComposition/AllCachingCmm.dfy
@@ -1,0 +1,115 @@
+// Copyright Amazon.com Inc. or its affiliates. All Rights Reserved.
+// SPDX-License-Identifier: Apache-2.0
+
+include "KeyDescriptionJson.dfy"
+include "AllRawAES.dfy"
+
+module {:options "-functionSyntax:4"} AllCachingCmm {
+  import opened JSON.Values
+  import opened KeyDescriptionJson
+  import opened Wrappers
+  import AllAlgorithmSuites
+  import AllRawAES
+  import SortedSets
+  import StandardLibrary
+
+  const StaticCashablePlaintextDataKey
+    := Object([
+                ("type", String("static-material-keyring")),
+                ("key", String("static-cashable-plaintext-data-key"))
+              ])
+
+  const StaticCashableAlgorithmSuite := AllAlgorithmSuites.AlgorithmSuites.GetESDKSuite(
+                                          AllAlgorithmSuites.Types.ALG_AES_256_GCM_HKDF_SHA512_COMMIT_KEY)
+
+  const StaticEncryptIdentifier := "+m9XmK8rzu0FLMlFmaElNNLcW7Cpp452Tcb/HepBGBbMR2DEfQBRroQbS6jq1acjpjx5hQ9GRKphCCy/ltmHFw=="
+  const StaticDecryptIdentifier := "Bghmwcshq6V3NOB77sSO/bmhGId6EoEVUfq+6MLKpW6YPccqlr/sqxL8R195Jn85LfSb66ovnnJcNmxanxnK+g=="
+
+
+  const Tests :=
+    (set
+       encrypt
+       <- set
+            cacheLimitTtlSeconds <- {5, 10, 12},
+            limitBytes <- {5, 10, 12},
+            limitMessages <- {5, 10, 12}
+            ::
+              Object([
+                       ("type", String("caching-cmm")),
+                       ("underlying", StaticCashablePlaintextDataKey),
+                       ("cacheLimitTtlSeconds", Number(Int(cacheLimitTtlSeconds))),
+                       ("limitBytes", Number(Int(limitBytes))),
+                       ("limitMessages", Number(Int(limitMessages))),
+                       ("getEntryIdentifier", String(StaticEncryptIdentifier)),
+                       ("putEntryIdentifier", String(StaticEncryptIdentifier))
+                     ]),
+       decrypt
+       <- set
+            cacheLimitTtlSeconds <- {5, 10, 12},
+            limitBytes <- {5, 10, 12},
+            limitMessages <- {5, 10, 12}
+            ::
+              Object([
+                       ("type", String("caching-cmm")),
+                       ("underlying", StaticCashablePlaintextDataKey),
+                       ("cacheLimitTtlSeconds", Number(Int(cacheLimitTtlSeconds))),
+                       ("limitBytes", Number(Int(limitBytes))),
+                       ("limitMessages", Number(Int(limitMessages))),
+                       ("getEntryIdentifier", String(StaticDecryptIdentifier)),
+                       ("putEntryIdentifier", String(StaticDecryptIdentifier))
+                     ])
+       ::
+         ToJson(
+         keyDescription := PositiveKeyDescriptionJSON(
+             description := "Successful caching test.",
+             encrypt := encrypt,
+             decrypt := decrypt
+           ),
+           algorithmSuite := StaticCashableAlgorithmSuite,
+           maxPlaintextLength := Some(5)
+         ))
+    + (set
+         encryptIdentifier <- {"", StaticEncryptIdentifier}
+         ::
+           ToJson(
+           keyDescription := NegativeEncryptKeyDescriptionJSON(
+               description := "Encrypt caching failure",
+               errorDescription := "The get or put will fail because the identifier is wrong.",
+               encrypt := Object([
+                                   ("type", String("caching-cmm")),
+                                   ("underlying", StaticCashablePlaintextDataKey),
+                                   ("cacheLimitTtlSeconds", Number(Int(5))),
+                                   ("getEntryIdentifier", String(encryptIdentifier)),
+                                   ("putEntryIdentifier", String(""))
+                                 ])
+             ),
+             algorithmSuite := StaticCashableAlgorithmSuite,
+             maxPlaintextLength := Some(5)
+           ))
+    + (set
+         decryptIdentifier <- {"", StaticDecryptIdentifier}
+         ::
+           ToJson(
+           keyDescription := NegativeDecryptKeyDescriptionJSON(
+               description := "Decrypt caching failure",
+               decryptErrorDescription := "The get or put will fail because the identifier is wrong.",
+               encrypt := Object([
+                                   ("type", String("caching-cmm")),
+                                   ("underlying", StaticCashablePlaintextDataKey),
+                                   ("cacheLimitTtlSeconds", Number(Int(5))),
+                                   ("getEntryIdentifier", String(StaticEncryptIdentifier))
+                                 ]),
+               decrypt := Object([
+                                   ("type", String("caching-cmm")),
+                                   ("underlying", StaticCashablePlaintextDataKey),
+                                   ("cacheLimitTtlSeconds", Number(Int(5))),
+                                   ("getEntryIdentifier", String(decryptIdentifier)),
+                                   ("putEntryIdentifier", String(""))
+                                 ])
+
+             ),
+             algorithmSuite := StaticCashableAlgorithmSuite,
+             maxPlaintextLength := Some(5)
+           ))
+
+}
