TestVectorsAwsCryptographicMaterialProviders/dafny/TestVectorsAwsCryptographicMaterialProviders/src/VectorsComposition/AllDefaultCmm.dfy
@@ -1,0 +1,159 @@
+// Copyright Amazon.com Inc. or its affiliates. All Rights Reserved.
+// SPDX-License-Identifier: Apache-2.0
+
+include "KeyDescriptionJson.dfy"
+include "AllRawAES.dfy"
+
+module {:options "-functionSyntax:4"} AllDefaultCmm {
+  import opened JSON.Values
+  import opened KeyDescriptionJson
+  import opened Wrappers
+  import AllAlgorithmSuites
+  import AllRawAES
+  import SortedSets
+  import StandardLibrary
+
+  const StaticNotPlaintextDataKey
+    := Object([
+                ("type", String("static-material-keyring")),
+                ("key", String("no-plaintext-data-key"))
+              ])
+  const StaticPlaintextDataKey
+    := Object([
+                ("type", String("static-material-keyring")),
+                ("key", String("static-plaintext-data-key"))
+              ])
+  const StaticAlgorithmSuite := AllAlgorithmSuites.AlgorithmSuites.GetESDKSuite(
+                                  AllAlgorithmSuites.Types.ALG_AES_128_GCM_IV12_TAG16_NO_KDF)
+
+  const AesKey := AllRawAES.aesPersistentKeyNames[|AllRawAES.aesPersistentKeyNames| - 1]
+  const RawAesKeyring
+    := Object([
+                ("type", String("raw")),
+                ("encryption-algorithm", String("aes")),
+                ("provider-id", String("aws-raw-vectors-persistent-" + AesKey)),
+                ("key", String(AesKey))
+              ])
+
+  function SubSets(ec: map<string, string>, keys: seq<string>)
+    : set<map<string, string>>
+    requires keys == SortedSets.ComputeSetToOrderedSequence2(ec.Keys, (a, b) => a < b)
+  {
+    if |ec| == 0 then
+      {map[]}
+    else
+      var subsets := SubSets(ec - {keys[0]}, keys[1..]);
+      subsets
+      + (set
+           s <- subsets
+           ::
+             s + map[keys[0] := ec[keys[0]]])
+  }
+
+  const SuccessTestingRequiredEncryptionContextKeysReproducedEncryptionContext :=
+    set
+      encryptionContext <- {map["a" := "a", "b" := "b"]},
+      requiredEncryptionContextKeys
+      <- set
+           s <- SubSets(
+                  encryptionContext,
+                  SortedSets.ComputeSetToOrderedSequence2(encryptionContext.Keys, (a, b) => a < b))
+           :: s.Keys,
+      reproducedEncryptionContext
+      <- set
+           s <- SubSets(
+                  encryptionContext,
+                  SortedSets.ComputeSetToOrderedSequence2(encryptionContext.Keys, (a, b) => a < b))
+           | s.Keys * requiredEncryptionContextKeys == requiredEncryptionContextKeys
+           :: s
+      ::
+        ToJson(
+        keyDescription := PositiveKeyDescriptionJSON(
+            description := "Success testing requiredEncryptionContextKeys/reproducedEncryptionContext",
+            encrypt := RawAesKeyring,
+            decrypt := RawAesKeyring
+          ),
+          algorithmSuite := StaticAlgorithmSuite,
+          encryptionContext := encryptionContext,
+          requiredEncryptionContextKeys := requiredEncryptionContextKeys,
+          reproducedEncryptionContext := Some(reproducedEncryptionContext)
+        )
+
+  const FailureBadReproducedEncryptionContext :=
+    set
+      encryptionContext <- {map["a" := "a", "b" := "b"]},
+      requiredEncryptionContextKeys
+      <- set
+           s <- SubSets(
+                  encryptionContext,
+                  SortedSets.ComputeSetToOrderedSequence2(encryptionContext.Keys, (a, b) => a < b))
+           :: s.Keys,
+      incorrectEncryptionContext
+      <- set
+           s <- SubSets(
+                  map["a" := "c", "b" := "c", "c" := "c"],
+                  SortedSets.ComputeSetToOrderedSequence2(map["a" := "c", "b" := "c", "c" := "c"].Keys, (a, b) => a < b))
+           | s != map[]
+           :: s,
+      reproducedEncryptionContext
+      <- set
+           s <- SubSets(
+                  encryptionContext,
+                  SortedSets.ComputeSetToOrderedSequence2(encryptionContext.Keys, (a, b) => a < b))
+           :: s + incorrectEncryptionContext
+      ::
+        ToJson(
+        keyDescription := NegativeDecryptKeyDescriptionJSON(
+            description := "Failure of reproducedEncryptionContext",
+            decryptErrorDescription := "The reproducedEncryptionContext is never correct",
+            encrypt := RawAesKeyring,
+            decrypt := RawAesKeyring
+          ),
+          algorithmSuite := StaticAlgorithmSuite,
+          encryptionContext := encryptionContext,
+          requiredEncryptionContextKeys := requiredEncryptionContextKeys,
+          reproducedEncryptionContext := Some(reproducedEncryptionContext)
+        )
+
+  const Tests :=
+    {
+      ToJson(
+      keyDescription := PositiveKeyDescriptionJSON(
+          description := "Simplest possible happy path",
+          encrypt := StaticPlaintextDataKey,
+          decrypt := StaticPlaintextDataKey
+        ),
+        algorithmSuite := StaticAlgorithmSuite
+      ),
+      ToJson(
+      keyDescription := NegativeEncryptKeyDescriptionJSON(
+          description := "Missing plaintext data key on encrypt",
+          errorDescription := "No plaintext data key on encrypt fails",
+          encrypt := StaticNotPlaintextDataKey
+        ),
+        algorithmSuite := StaticAlgorithmSuite
+      ),
+      ToJson(
+      keyDescription := NegativeDecryptKeyDescriptionJSON(
+          description := "Missing plaintext data key on decrypt",
+          decryptErrorDescription := "No plaintext data key on encrypt fails",
+          encrypt := StaticPlaintextDataKey,
+          decrypt := StaticNotPlaintextDataKey
+        ),
+        algorithmSuite := StaticAlgorithmSuite
+      ),
+      ToJson(
+      keyDescription := NegativeEncryptKeyDescriptionJSON(
+          description := "Missing plaintext data key on encrypt",
+          errorDescription := "No plaintext data key on encrypt fails",
+          encrypt := StaticPlaintextDataKey
+        ),
+        algorithmSuite := StaticAlgorithmSuite,
+        encryptionContext := map["a" := "a", "b" := "b"],
+        requiredEncryptionContextKeys := {"c"}
+      )
+    }
+    + FailureBadReproducedEncryptionContext
+    + SuccessTestingRequiredEncryptionContextKeysReproducedEncryptionContext
+
+}
