TestVectorsAwsCryptographicMaterialProviders/dafny/TestVectorsAwsCryptographicMaterialProviders/src/VectorsComposition/AllHierarchy.dfy
@@ -1,0 +1,34 @@
+// Copyright Amazon.com Inc. or its affiliates. All Rights Reserved.
+// SPDX-License-Identifier: Apache-2.0
+
+include "KeyDescriptionJson.dfy"
+
+module {:options "-functionSyntax:4"} AllHierarchy {
+  import opened JSON.Values
+  import opened KeyDescriptionJson
+
+  const AllHierarchy :=
+    set
+      keyId <- [ "static-branch-key-1" ]
+      ::
+        PositiveKeyDescriptionJSON(
+          description := "Hierarchy KMS " + keyId,
+          encrypt := Object([
+                              ("type", String("aws-kms-hierarchy")),
+                              ("key", String(keyId))
+                            ]),
+          decrypt := Object([
+                              ("type", String("aws-kms-hierarchy")),
+                              ("key", String(keyId))
+                            ])
+        )
+
+  const Tests :=
+    set
+      keyDescription <- AllHierarchy,
+      algorithmSuite <- AllAlgorithmSuites.AllAlgorithmSuites
+      :: ToJson(
+           keyDescription := keyDescription,
+           algorithmSuite := algorithmSuite
+         )
+}
