TestVectorsAwsCryptographicMaterialProviders/dafny/TestVectorsAwsCryptographicMaterialProviders/src/VectorsComposition/AllKms.dfy
@@ -1,0 +1,33 @@
+// Copyright Amazon.com Inc. or its affiliates. All Rights Reserved.
+// SPDX-License-Identifier: Apache-2.0
+
+include "KeyDescriptionJson.dfy"
+
+module {:options "-functionSyntax:4"} AllKms {
+  import opened JSON.Values
+  import opened KeyDescriptionJson
+
+  const AllAwsKMSKeys := [ "us-west-2-decryptable", "us-west-2-mrk" ]
+  const AllKms :=
+    set
+      key <- AllAwsKMSKeys
+      ::
+        var keyDescription := Object([
+                                       ("type", String("aws-kms")),
+                                       ("key", String(key))
+                                     ]);
+        PositiveKeyDescriptionJSON(
+          description := "Generated KMS " + key,
+          encrypt := keyDescription,
+          decrypt := keyDescription
+        )
+
+  const Tests :=
+    set
+      keyDescription <- AllKms,
+      algorithmSuite <- AllAlgorithmSuites.AllAlgorithmSuites
+      :: ToJson(
+           keyDescription := keyDescription,
+           algorithmSuite := algorithmSuite
+         )
+}
