TestVectorsAwsCryptographicMaterialProviders/dafny/TestVectorsAwsCryptographicMaterialProviders/src/VectorsComposition/AllKmsMrkAware.dfy
@@ -1,0 +1,37 @@
+// Copyright Amazon.com Inc. or its affiliates. All Rights Reserved.
+// SPDX-License-Identifier: Apache-2.0
+
+include "KeyDescriptionJson.dfy"
+
+module {:options "-functionSyntax:4"} AllKmsMrkAware {
+  import Types = AwsCryptographyMaterialProvidersTypes
+  import opened JSON.Values
+  import opened KeyDescriptionJson
+
+  const AllAwsKMSMrkKeys := [ "us-west-2-mrk", "us-east-1-mrk" ]
+  const AllKmsMrkAware :=
+    set
+      encryptKey <- AllAwsKMSMrkKeys,
+      decryptKey <- AllAwsKMSMrkKeys
+      ::
+        PositiveKeyDescriptionJSON(
+          description := "Generated KMS MRK " + encryptKey + "->" + decryptKey,
+          encrypt := Object([
+                              ("type", String("aws-kms-mrk-aware")),
+                              ("key", String(encryptKey))
+                            ]),
+          decrypt := Object([
+                              ("type", String("aws-kms-mrk-aware")),
+                              ("key", String(decryptKey))
+                            ])
+        )
+
+  const Tests :=
+    set
+      keyDescription <- AllKmsMrkAware,
+      algorithmSuite <- AllAlgorithmSuites.AllAlgorithmSuites
+      :: ToJson(
+           keyDescription := keyDescription,
+           algorithmSuite := algorithmSuite
+         )
+}
