TestVectorsAwsCryptographicMaterialProviders/dafny/TestVectorsAwsCryptographicMaterialProviders/src/VectorsComposition/AllKmsMrkAwareDiscovery.dfy
@@ -1,0 +1,69 @@
+// Copyright Amazon.com Inc. or its affiliates. All Rights Reserved.
+// SPDX-License-Identifier: Apache-2.0
+
+include "KeyDescriptionJson.dfy"
+include "AllKmsMrkAware.dfy"
+
+module {:options "-functionSyntax:4"} AllKmsMrkAwareDiscovery {
+  import Types = AwsCryptographyMaterialProvidersTypes
+  import Seq
+  import opened Wrappers
+  import opened JSON.Values
+  import opened KeyDescriptionJson
+  import AllKmsMrkAware
+  import AllAlgorithmSuites
+
+  // These values MUST correspond to the KMS keys above
+  // At this time, this list is simplistic
+  const AwsPartitions := [ "aws" ]
+  const AWSAccounts := [ "658956600833" ]
+  const AllDiscoveryFilters: set<Option<Types.DiscoveryFilter>> := {
+    Some(Types.DiscoveryFilter(
+           partition := "aws",
+           accountIds := [ "658956600833" ]
+         )),
+    None
+  }
+
+  const AllKmsMrkAwareDiscovery :=
+    set
+      keyId <- AllKmsMrkAware.AllAwsKMSMrkKeys,
+      filter <- AllDiscoveryFilters
+      ::
+        PositiveKeyDescriptionJSON(
+          description := "Discovery KMS MRK " + keyId +
+          "->" + if filter.Some? then
+            "Filter " + filter.value.partition + " " + Seq.Flatten(filter.value.accountIds)
+          else
+            "No Filter"
+        ,
+          encrypt := Object([
+                              ("type", String("aws-kms-mrk-aware")),
+                              ("key", String(keyId))
+                            ]),
+          decrypt := if filter.Some? then
+            Object([
+                     ("type", String("aws-kms-mrk-aware-discovery")),
+                     ("default-mrk-region", String("us-west-2")),
+                     ("aws-kms-discovery-filter", Object(
+                      [
+                      ("partition", String(filter.value.partition)),
+                      ("account-ids", Array(
+                      Seq.Map(s => String(s), filter.value.accountIds)))
+                      ]))
+                   ])
+          else
+            Object([
+                     ("type", String("aws-kms-mrk-aware-discovery")),
+                     ("default-mrk-region", String("us-west-2"))])
+        )
+
+  const Tests :=
+    set
+      keyDescription <- AllKmsMrkAwareDiscovery,
+      algorithmSuite <- AllAlgorithmSuites.AllAlgorithmSuites
+      :: ToJson(
+           keyDescription := keyDescription,
+           algorithmSuite := algorithmSuite
+         )
+}
