TestVectorsAwsCryptographicMaterialProviders/dafny/TestVectorsAwsCryptographicMaterialProviders/src/VectorsComposition/AllKmsRsa.dfy
@@ -1,0 +1,47 @@
+// Copyright Amazon.com Inc. or its affiliates. All Rights Reserved.
+// SPDX-License-Identifier: Apache-2.0
+
+include "KeyDescriptionJson.dfy"
+
+module {:options "-functionSyntax:4"} AllKmsRsa {
+  import ComAmazonawsKmsTypes
+  import opened JSON.Values
+  import opened KeyDescriptionJson
+
+  const AllEncryptionAlgorithmSpec :=
+    set e: ComAmazonawsKmsTypes.EncryptionAlgorithmSpec
+      | !e.SYMMETRIC_DEFAULT?
+      :: match e
+         case RSAES_OAEP_SHA_1() => "RSAES_OAEP_SHA_1"
+         case RSAES_OAEP_SHA_256() => "RSAES_OAEP_SHA_256"
+  const AllKmsRsaKeys := [ "us-west-2-rsa-mrk" ]
+  const KmsRsa := "KMS RSA "
+
+  const AllKmsRsa :=
+    set
+      keyId <- AllKmsRsaKeys,
+      algorithmSpec <- AllEncryptionAlgorithmSpec
+      ::
+        PositiveKeyDescriptionJSON(
+          description := KmsRsa + keyId,
+          encrypt := Object([
+                              ("type", String("aws-kms-rsa")),
+                              ("key", String(keyId)),
+                              ("encryption-algorithm", String(algorithmSpec))
+                            ]),
+          decrypt := Object([
+                              ("type", String("aws-kms-rsa")),
+                              ("key", String(keyId)),
+                              ("encryption-algorithm", String(algorithmSpec))
+                            ])
+        )
+
+  const Tests :=
+    set
+      keyDescription <- AllKmsRsa,
+      algorithmSuite <- AllAlgorithmSuites.AllAlgorithmSuites
+      :: ToJson(
+           keyDescription := keyDescription,
+           algorithmSuite := algorithmSuite
+         )
+}
