TestVectorsAwsCryptographicMaterialProviders/dafny/TestVectorsAwsCryptographicMaterialProviders/src/VectorsComposition/AllRawAES.dfy
@@ -1,0 +1,37 @@
+// Copyright Amazon.com Inc. or its affiliates. All Rights Reserved.
+// SPDX-License-Identifier: Apache-2.0
+
+include "KeyDescriptionJson.dfy"
+
+module {:options "-functionSyntax:4"} AllRawAES {
+  import Types = AwsCryptographyMaterialProvidersTypes
+  import opened JSON.Values
+  import opened KeyDescriptionJson
+
+  // These are all the PositiveKeyDescription for the RawAESKeyring
+  const aesPersistentKeyNames := [ "aes-128", "aes-192", "aes-256"]
+  const AllRawAES :=
+    set
+      key <- aesPersistentKeyNames
+      ::
+        var keyDescription := Object([
+                                       ("type", String("raw")),
+                                       ("encryption-algorithm", String("aes")),
+                                       ("provider-id", String("aws-raw-vectors-persistent-" + key)),
+                                       ("key", String(key))
+                                     ]);
+        PositiveKeyDescriptionJSON(
+          description := "Generated RawAES " + key,
+          encrypt := keyDescription,
+          decrypt := keyDescription
+        )
+
+  const Tests :=
+    set
+      keyDescription <- AllRawAES,
+      algorithmSuite <- AllAlgorithmSuites.AllAlgorithmSuites
+      :: ToJson(
+           keyDescription := keyDescription,
+           algorithmSuite := algorithmSuite
+         )
+}
