TestVectorsAwsCryptographicMaterialProviders/dafny/TestVectorsAwsCryptographicMaterialProviders/src/VectorsComposition/AllRawRSA.dfy
@@ -1,0 +1,62 @@
+// Copyright Amazon.com Inc. or its affiliates. All Rights Reserved.
+// SPDX-License-Identifier: Apache-2.0
+
+include "KeyDescriptionJson.dfy"
+
+module {:options "-functionSyntax:4"} AllRawRSA {
+  import Types = AwsCryptographyMaterialProvidersTypes
+  import opened JSON.Values
+  import opened KeyDescriptionJson
+
+  // These are all the PositiveKeyDescription for the RawRSAKeyring
+  const rsaPersistentKeyNamesWithoutPublicPrivate := [ "rsa-4096" ]
+  const AllRawRSA :=
+    set
+      key <- rsaPersistentKeyNamesWithoutPublicPrivate,
+             padding: Types.PaddingScheme
+      ::
+        var sharedOptions := [
+                               ("type", String("raw")),
+                               ("encryption-algorithm", String("rsa")),
+                               ("provider-id", String("aws-raw-vectors-persistent-" + key)),
+                               ("padding-algorithm", String(match padding
+                                case PKCS1() => "pkcs1"
+                                case _ => "oaep-mgf1"
+                                )),
+                               ("padding-hash", String(match padding
+                                case PKCS1() => "sha1"
+                                case OAEP_SHA1_MGF1() => "sha1"
+                                case OAEP_SHA256_MGF1() => "sha256"
+                                case OAEP_SHA384_MGF1() => "sha384"
+                                case OAEP_SHA512_MGF1() => "sha512"
+                                ))
+                             ];
+        PositiveKeyDescriptionJSON(
+          description := "Generated RawRSA " + key + " "
+          + match padding
+            case PKCS1() => "pkcs1-sha1"
+            case OAEP_SHA1_MGF1() => "oaep-mgf1-sha1"
+            case OAEP_SHA256_MGF1() => "oaep-mgf1-sha256"
+            case OAEP_SHA384_MGF1() => "oaep-mgf1-sha384"
+            case OAEP_SHA512_MGF1() => "oaep-mgf1-sha512"
+        ,
+          encrypt := Object(
+            sharedOptions +
+            [("key", String(key + "-public"))]
+          ),
+          decrypt := Object(
+            sharedOptions +
+            [("key", String(key + "-private"))]
+          )
+        )
+
+  const Tests :=
+    set
+      keyDescription <- AllRawRSA,
+      algorithmSuite <- AllAlgorithmSuites.AllAlgorithmSuites
+      :: ToJson(
+           keyDescription := keyDescription,
+           algorithmSuite := algorithmSuite
+         )
+
+}
