TestVectorsAwsCryptographicMaterialProviders/dafny/TestVectorsAwsCryptographicMaterialProviders/src/VectorsComposition/KeyDescriptionJson.dfy
@@ -1,0 +1,108 @@
+// Copyright Amazon.com Inc. or its affiliates. All Rights Reserved.
+// SPDX-License-Identifier: Apache-2.0
+
+include "../JSONHelpers.dfy"
+include "AllAlgorithmSuites.dfy"
+
+module {:options "-functionSyntax:4"} KeyDescriptionJson {
+  import opened JSON.Values
+  import AllAlgorithmSuites
+  import AllAlgorithmSuites.Types
+  import opened Wrappers
+  import SortedSets
+  import Seq
+  import StandardLibrary
+
+  datatype KeyDescriptionJSON =
+    | PositiveKeyDescriptionJSON(
+        description: string,
+        encrypt: JSON,
+        decrypt: JSON
+      )
+    | NegativeDecryptKeyDescriptionJSON(
+        description: string,
+        decryptErrorDescription: string,
+        encrypt: JSON,
+        decrypt: JSON
+      )
+    | NegativeEncryptKeyDescriptionJSON(
+        description: string,
+        errorDescription: string,
+        encrypt: JSON
+      )
+
+  function ToJson(
+    nameonly keyDescription: KeyDescriptionJSON,
+    nameonly algorithmSuite: Types.AlgorithmSuiteInfo,
+    nameonly encryptionContext: map<string, string> := map[],
+    nameonly requiredEncryptionContextKeys: set<string> := {},
+    nameonly reproducedEncryptionContext: Option<map<string, string>> := None,
+    nameonly maxPlaintextLength: Option<nat> := None
+  )
+    : JSON
+    requires keyDescription.NegativeEncryptKeyDescriptionJSON? ==> reproducedEncryptionContext.None?
+  {
+    var id := AllAlgorithmSuites.ToHex(algorithmSuite);
+    var reproducedEc
+      := if reproducedEncryptionContext.Some? then
+           [("reproducedEncryptionContext",
+             EncryptionContextToJson(reproducedEncryptionContext.value))]
+         else
+           [];
+
+    var maxPlaintextL
+      := if maxPlaintextLength.Some? then
+           [("maxPlaintextLength",
+             Number(Int(maxPlaintextLength.value)))]
+         else
+           [];
+    match keyDescription
+    case PositiveKeyDescriptionJSON(description, encrypt, decrypt) =>
+      Object([
+               ("type", String("positive-keyring")),
+               ("description", String(description + " " + id)),
+               ("algorithmSuiteId", String(id)),
+               ("encryptionContext", EncryptionContextToJson(encryptionContext)),
+               ("requiredEncryptionContextKeys", EncryptionContextKeysToJson(requiredEncryptionContextKeys)),
+               ("encryptKeyDescription", encrypt),
+               ("decryptKeyDescription", decrypt)
+             ] + reproducedEc + maxPlaintextL)
+    case NegativeEncryptKeyDescriptionJSON(description, errorDescription, encrypt) =>
+      Object([
+               ("type", String("negative-encrypt-keyring")),
+               ("description", String(description + " " + id)),
+               ("errorDescription", String(errorDescription)),
+               ("algorithmSuiteId", String(id)),
+               ("encryptionContext", EncryptionContextToJson(encryptionContext)),
+               ("requiredEncryptionContextKeys", EncryptionContextKeysToJson(requiredEncryptionContextKeys)),
+               ("keyDescription", encrypt)
+             ] + maxPlaintextL)
+    case NegativeDecryptKeyDescriptionJSON(description, errorDescription, encrypt, decrypt) =>
+      Object([
+               ("type", String("negative-decrypt-keyring")),
+               ("description", String(description + " " + id)),
+               ("decryptErrorDescription", String(errorDescription)),
+               ("algorithmSuiteId", String(id)),
+               ("encryptionContext", EncryptionContextToJson(encryptionContext)),
+               ("requiredEncryptionContextKeys", EncryptionContextKeysToJson(requiredEncryptionContextKeys)),
+               ("encryptKeyDescription", encrypt),
+               ("decryptKeyDescription", decrypt)
+             ] + reproducedEc + maxPlaintextL)
+  }
+
+  function EncryptionContextKeysToJson(keys: set<string>)
+    : JSON
+  {
+    var k := SortedSets.ComputeSetToSequence(keys);
+    Array(seq(|k|, i requires 0 <= i < |k| => String(k[i])))
+  }
+
+  function EncryptionContextToJson(m: map<string, string>)
+    : JSON
+  {
+    var keys := SortedSets.ComputeSetToSequence(m.Keys);
+    var pairsBytes := Seq.Map(k requires k in m.Keys => (k, String(m[k])), keys);
+    Object(pairsBytes)
+  }
+
+}
